tweaking hoare shallow

examples/metatheory/hoare-shallow.fst
@@ -1,3 +1,8 @@
+(*--build-config
+    options:--admit_fsi Set;
+    variables:LIB=../../lib;
+    other-files:$LIB/ext.fst $LIB/set.fsi $LIB/heap.fst $LIB/st.fst
+  --*)
 module While
 open Heap
 open ST
@@ -9,18 +14,18 @@ effect com (a:Type) (p:Asrt) (q:Asrt) = St a (fun h' -> p h')
 
 type com' (p:Asrt) (q:Asrt) = unit -> com unit p q
 
-val skip : p:Asrt -> com unit p p 
+val skip : p:Asrt -> com unit p p
 let skip (p:Asrt) = ()
 
 type exp (a:Type) (p:Asrt) (q:(a -> Asrt)) =
-       unit -> St a (fun h0 -> p h0) (fun h0 x h1 -> h0=h1 /\ q x h1) 
+       unit -> St a (fun h0 -> p h0) (fun h0 x h1 -> h0=h1 /\ q x h1)
 
 (* Using equality constraints for better type inference *)
 val _while: p:Asrt -> q:(bool -> Asrt)
         -> =guard:exp bool p q
         -> =body:(unit -> com unit (fun h -> p h /\ q true h) p)
         -> com unit p (fun h -> p h /\ q false h)
-let rec _while guard body = 
+let rec _while guard body =
   if guard () then (body (); _while guard body)
 
 val cond: p:Asrt -> q:(bool -> Asrt) -> r:Asrt -> s:Asrt
@@ -29,47 +34,72 @@ val cond: p:Asrt -> q:(bool -> Asrt) -> r:Asrt -> s:Asrt
       -> =_else:(unit -> com unit (fun h -> q false h) s)
       -> com unit p (fun h -> r h \/ s h)
 (* Loss in precision here, since com does not include 2-state post-conditions *)
-let cond guard _then _else = 
+let cond guard _then _else =
   if guard()
   then _then()
   else _else()
 
+
+(* Another way to recover precision is to go WP style *)
+val condWP: p:Asrt -> q:(bool -> Asrt)
+        -> pre1:Asrt -> pre2:Asrt -> post:Asrt
+        -> =guard:exp bool p q
+        -> =_then:(unit -> com unit pre1 post)
+        -> =_else:(unit -> com unit pre2 post)
+        -> com unit (fun h -> p h
+                            /\ (q true h ==> pre1 h)
+                            /\ (q false h ==> pre2 h))
+                    post
+let condWP guard _then _else =
+    if guard()
+    then _then()
+    else _else()
+
+val write': a:Type -> p:Asrt -> r:ref a -> v:a
+          -> com unit (fun h -> p (upd h r v))
+                      p
+let write' r v = r := v
+
+val read': a:Type -> p:(a -> Asrt) -> r:ref a -> Tot (exp a (fun h -> p (sel h r) h) p)
+let read' r () = !r
+
+(* Yet another way is to break out of com and drop into F*'s St *)
 val cond2: p:Asrt -> q:(bool -> Asrt) -> r:Asrt -> s:Asrt
       -> =guard:exp bool p q
       -> =_then:(unit -> com unit (fun h -> q true h) r)
       -> =_else:(unit -> com unit (fun h -> q false h) s)
-      -> St unit p (fun h0 _ h1 -> 
+      -> St unit p (fun h0 _ h1 ->
                       (q true h0 /\ r h1)
                    \/ (q false h0 /\ s h1))
-(* recover precision by dropping back into St *)
-let cond2 guard _then _else = 
+let cond2 guard _then _else =
   if guard()
   then _then()
   else _else()
 
-(* CH: In Hoare logic this is actually even less precise (r = s);
+(* CH: For the record:
+      In Hoare logic this is actually even less precise (r = s);
        one has to use explicit weakening *)
 val cond3: p:Asrt -> q:(bool -> Asrt) -> r:Asrt
       -> =guard:exp bool p q
       -> =_then:(unit -> com unit (fun h -> q true h) r)
       -> =_else:(unit -> com unit (fun h -> q false h) r)
       -> com unit p (fun h -> r h)
-let cond3 guard _then _else = 
+let cond3 guard _then _else =
   if guard()
   then _then()
   else _else()
 
 
 (* A sample program written against this API *)
-logic type pre (r1:ref int) (r2:ref int) (h:heap) = 
-          (contains h r1 
+logic type pre (r1:ref int) (r2:ref int) (h:heap) =
+          (contains h r1
            /\ contains h r2
            /\ sel h r1 <= sel h r2)
 
-logic type post  (r1:ref int) (r2:ref int) (b:bool) (h:heap) = 
+logic type post  (r1:ref int) (r2:ref int) (b:bool) (h:heap) =
           (b = (sel h r1 <> sel h r2))
 
-(* equalize r1 r2: 
+(* equalize r1 r2:
    requires the contents of r1 to be less than or equal to r2
             Repeatedly increments r1
    ensures the contents of r1 is equal to to r2
@@ -85,13 +115,13 @@ let equalize r1 r2 =
     fun () -> read r1 <> read r2 in
 
   let body : unit -> com unit (fun h -> pre r1 r2 h /\ post r1 r2 true h)
-                              (pre r1 r2) = 
+                              (pre r1 r2) =
     fun () -> write r1 (read r1 + 1) in
 
   _while test body
 
 (* Exercise:
 
-     Relax the pre-condition that r1 is less than or equal to r2 
+     Relax the pre-condition that r1 is less than or equal to r2
      so that it works with any pair of refs.
 *)
