lib/mref.fst
@@ -12,8 +12,9 @@ type stable : #a:Type -> (a -> Type) -> Reln a -> Type =
   fun (a:Type) (p:(a -> Type)) (b:Reln a) ->
     (forall x y. p x /\ b x y ==> p y)
 
-(*private*) type mref (a:Type) (b:Reln a) = ref a
-(*private*) type token : #a:Type -> #b:Reln a -> mref a b -> (a -> Type) -> Type =
+(*private*)
+type mref (a:Type) (b:Reln a) = ref a
+opaque logic type token : #a:Type -> #b:Reln a -> mref a b -> (a -> Type) -> Type =
   fun (a:Type) (b:Reln a) (r:mref a b) (p:a -> Type) -> unit
 
 let fresh x h0 r h1 = not(contains h0 r) && contains h1 r && h1=upd h0 r x
@@ -48,15 +49,15 @@ val witness: #a:Type
           -> #b:Reln a
           -> m:mref a b
           -> p:(a -> Type)
-          -> St (u:unit {token m p})
+          -> St unit
                 (requires (fun h0 -> p (sel h0 m) /\ stable p b))
-                (ensures (fun h0 _ h1 -> h0=h1))
+                (ensures (fun h0 _ h1 -> h0=h1 /\ token m p))
 let witness (a:Type) (b:Reln a) m (p: a -> Type) = ()
 
 assume val recall: a:Type
                 -> b:Reln a
-                -> p:(a -> Type) 
-                -> m:mref a b {token m p}
+                -> m:mref a b
+                -> p:(a -> Type)
                 -> St unit
-                      (requires (fun _ -> True))
+                      (requires (fun _ ->  token m p))
                       (ensures (fun h0 _ h1 -> h0=h1 /\ p (sel h1 m)))
